fixing expression unification. working on verification.

src/SepExpr.v
@@ -3,23 +3,16 @@ Require Import SepTheoryX PropX.
 Require Import PropXTac.
 Require Import RelationClasses EqdepClass.
 Require Import Expr.
-Require Import DepList.
 Require Import Setoid.
 
 Set Implicit Arguments.
 Set Strict Implicit.
 
-Require NatMap Multimap.
-
-Module FM := NatMap.IntMap.
-Module MM := Multimap.Make FM.
-Module MF := NatMap.MoreFMapFacts FM.
-
 Definition BadInj types (e : expr types) := False.
 Definition BadPred (f : func) := False.
 Definition BadPredApply types (f : func) (es : list (expr types)) (_ : env types) := False.
 
-Module Type SepExprType.
+Module Type SepExpr.
   Declare Module ST : SepTheoryX.SepTheoryXType.
 
   Section env.
@@ -86,41 +79,290 @@ Module Type SepExprType.
 
     End funcs_preds.
 
-    Record SHeap : Type :=
-    { impures : MM.mmap (exprs types)
-    ; pures   : list (expr types)
-    ; other   : list (ST.hprop (tvarD types pcType) (tvarD types stateType) nil)
-    }.
-
-    Parameter star_SHeap : SHeap -> SHeap -> SHeap.
-
-    Parameter sheapSubstU : nat -> nat -> nat -> SHeap -> SHeap.
-
-    Parameter hash : sexpr -> variables * SHeap.
-
-
-    (** TODO: What happens if I denote this directly to hprop?
-     ** - fewer lemmas about concrete syntax!
-     ** - can't re-hash (probably don't want to do this anyways...)
-     ** * I think this is Ok for now
-     **)
-    Parameter sheapD : SHeap -> sexpr.
-
     Fixpoint existsEach (ls : list tvar) {struct ls} : sexpr -> sexpr :=
       match ls with
         | nil => fun x => x
         | t :: ts => fun y => Exists t (@existsEach ts y)
       end.
 
-    Parameter sheap_liftVars : nat -> nat -> SHeap -> SHeap.
+  End env.
+
+  Implicit Arguments Emp [ types pcType stateType ].
+  Implicit Arguments Star [ types pcType stateType ].
+  Implicit Arguments Exists [ types pcType stateType ].
+  Implicit Arguments Func [ types pcType stateType ].
+  Implicit Arguments Const [ types pcType stateType ].
+  Implicit Arguments Inj [ types pcType stateType ].
+
+End SepExpr.
+
+Module SepExprFacts (SE : SepExpr).
+  Module SEP_FACTS := SepTheoryX_Rewrites SE.ST.
+
+  Section env.
+    Variable types : list type.
+    Variable pcType : tvar.
+    Variable stateType : tvar.
+    Variable funcs : functions types.
+    Variable preds : SE.predicates types pcType stateType.
+    
+    Variables U G : env types.
+    Variable cs : codeSpec (tvarD types pcType) (tvarD types stateType).
+
+    Global Instance Trans_himp : Transitive (@SE.himp types _ _ funcs preds U G cs).
+    Proof.
+      red. unfold SE.himp. intros; etransitivity; eauto.
+    Qed.
+
+    Global Instance Trans_heq : Transitive (@SE.heq types _ _ funcs preds U G cs).
+    Proof.
+      red. unfold SE.heq. intros; etransitivity; eauto.
+    Qed.
+
+    Global Instance Refl_himp : Reflexive (@SE.himp types _ _ funcs preds U G cs).
+    Proof.
+      red; unfold SE.himp; intros. reflexivity.
+    Qed.
+
+    Global Instance Refl_heq : Reflexive (@SE.heq types _ _ funcs preds U G cs).
+    Proof.
+      red; unfold SE.heq; intros. reflexivity.
+    Qed.
+
+    Global Instance Sym_heq : Symmetric (@SE.heq types _ _ funcs preds U G cs).
+    Proof.
+      red; unfold SE.heq; intros. symmetry. auto.    
+    Qed.
+
+    Global Instance Equiv_heq : Equivalence (SE.heq funcs preds U G cs).
+    Proof.
+      constructor; eauto with typeclass_instances.
+    Qed.
+
+    Add Parametric Relation : (@SE.sexpr types pcType stateType) (@SE.himp types _ _ funcs preds U G cs)
+      reflexivity proved by  Refl_himp
+      transitivity proved by Trans_himp
+    as himp_rel.
+
+    Add Parametric Relation : (@SE.sexpr types pcType stateType) (@SE.heq types _ _ funcs preds U G cs)
+      reflexivity proved by  Refl_heq
+      symmetry proved by Sym_heq
+      transitivity proved by Trans_heq
+    as heq_rel.
+
+    Global Add Parametric Morphism : (@SE.Star types pcType stateType) with
+      signature (SE.himp funcs preds U G cs ==> SE.himp funcs preds U G cs ==> SE.himp funcs preds U G cs)      
+      as star_himp_mor.
+    Proof.
+      unfold SE.himp; simpl; intros; eapply SEP_FACTS.star_himp_mor; eauto.
+    Qed.
+
+    Global Add Parametric Morphism : (@SE.Star types pcType stateType) with
+      signature (SE.heq funcs preds U G cs ==> SE.heq funcs preds U G cs ==> SE.heq funcs preds U G cs)      
+      as star_heq_mor.
+    Proof.
+      unfold SE.himp; simpl; intros; eapply SEP_FACTS.star_heq_mor; eauto.
+    Qed.
+
+    Global Add Parametric Morphism : (SE.himp funcs preds U G cs) with 
+      signature (SE.heq funcs preds U G cs ==> SE.heq funcs preds U G cs ==> Basics.impl)
+      as himp_heq_mor.
+    Proof.
+      unfold SE.heq; simpl; intros. eapply SEP_FACTS.himp_heq_mor; eauto.
+    Qed.
+
+    Global Add Parametric Morphism : (SE.himp funcs preds U G cs) with 
+      signature (SE.himp funcs preds U G cs --> SE.himp funcs preds U G cs ++> Basics.impl)
+      as himp_himp_mor.
+    Proof.
+      unfold SE.himp; simpl; intros. eapply SEP_FACTS.himp_himp_mor; eauto.
+    Qed.
+
+    Global Add Parametric Morphism : (SE.sexprD funcs preds U G) with 
+      signature (SE.heq funcs preds U G cs ==> SE.ST.heq cs)
+      as heq_ST_heq_mor.
+    Proof.
+      unfold SE.heq; simpl; auto.
+    Qed.
+
+    Lemma heq_star_emp_r : forall P, 
+      SE.heq funcs preds U G cs (SE.Star P SE.Emp) P.
+    Proof.
+      unfold SE.heq; simpl; intros; autorewrite with hprop; reflexivity.
+    Qed.
+
+    Lemma heq_star_emp_l : forall P, 
+      SE.heq funcs preds U G cs (SE.Star SE.Emp P) P.
+    Proof.
+      unfold SE.heq; simpl; intros; autorewrite with hprop; reflexivity.
+    Qed.
+
+    Lemma heq_star_assoc : forall P Q R, 
+      SE.heq funcs preds U G cs (SE.Star (SE.Star P Q) R) (SE.Star P (SE.Star Q R)).
+    Proof.
+      unfold SE.heq; simpl; intros; autorewrite with hprop. rewrite SE.ST.heq_star_assoc. reflexivity.
+    Qed.
+
+    Lemma heq_star_comm : forall P Q, 
+      SE.heq funcs preds U G cs (SE.Star P Q) (SE.Star Q P).
+    Proof.
+      unfold SE.heq; simpl; intros; apply SE.ST.heq_star_comm.
+    Qed.
+
+    Lemma heq_star_frame : forall P Q R S, 
+      SE.heq funcs preds U G cs P R ->
+      SE.heq funcs preds U G cs Q S ->
+      SE.heq funcs preds U G cs (SE.Star P Q) (SE.Star R S).
+    Proof.
+      unfold SE.heq; simpl; intros. eapply SE.ST.heq_star_frame; auto.
+    Qed.
+    
+    Lemma himp_star_frame : forall P Q R S,
+      SE.himp funcs preds U G cs P R ->
+      SE.himp funcs preds U G cs Q S ->
+      SE.himp funcs preds U G cs (SE.Star P Q) (SE.Star R S).
+    Proof.
+      unfold SE.himp; simpl; intros. rewrite H; rewrite H0; reflexivity.
+    Qed.
+    
+    Lemma heq_star_comm_p : forall P Q R,
+      SE.heq funcs preds U G cs (SE.Star P Q) R ->
+      SE.heq funcs preds U G cs (SE.Star Q P) R.
+    Proof.
+      intros. rewrite heq_star_comm. auto.
+    Qed.
+
+    Lemma heq_star_comm_c : forall P Q R,
+      SE.heq funcs preds U G cs R (SE.Star P Q) ->
+      SE.heq funcs preds U G cs R (SE.Star Q P).
+    Proof.
+      intros. rewrite heq_star_comm. auto.
+    Qed.
+
+    Lemma heq_star_assoc_p1 : forall P Q R S,
+      SE.heq funcs preds U G cs (SE.Star P (SE.Star Q R)) S ->
+      SE.heq funcs preds U G cs (SE.Star (SE.Star P Q) R) S.
+    Proof.
+      intros. rewrite heq_star_assoc; auto.
+    Qed.
+
+    Lemma heq_star_assoc_p2 : forall P Q R S,
+      SE.heq funcs preds U G cs (SE.Star Q (SE.Star P R)) S ->
+      SE.heq funcs preds U G cs (SE.Star (SE.Star P Q) R) S.
+    Proof.
+      intros. apply heq_star_assoc_p1 in H. rewrite <- H.
+      apply heq_star_frame; try reflexivity. rewrite heq_star_comm. reflexivity.
+    Qed.
+
+    Lemma heq_star_assoc_c1 : forall P Q R S,
+      SE.heq funcs preds U G cs S (SE.Star P (SE.Star Q R)) ->
+      SE.heq funcs preds U G cs S (SE.Star (SE.Star P Q) R).
+    Proof.
+      intros. rewrite heq_star_assoc; auto.
+    Qed.
+
+    Lemma heq_star_assoc_c2 : forall P Q R S,
+      SE.heq funcs preds U G cs S (SE.Star Q (SE.Star P R)) ->
+      SE.heq funcs preds U G cs S (SE.Star (SE.Star P Q) R).
+    Proof.
+      intros. apply heq_star_assoc_c1 in H. rewrite H.
+      apply heq_star_frame; try reflexivity. apply heq_star_comm; reflexivity.
+    Qed.
+
+    Lemma heq_star_emp_p : forall P S,
+      SE.heq funcs preds U G cs P S ->
+      SE.heq funcs preds U G cs (SE.Star SE.Emp P) S.
+    Proof.
+      intros. rewrite heq_star_emp_l. auto.
+    Qed.
+
+    Lemma heq_star_emp_c : forall P S,
+      SE.heq funcs preds U G cs S P ->
+      SE.heq funcs preds U G cs S (SE.Star SE.Emp P).
+    Proof.
+      intros. rewrite heq_star_emp_l. auto.
+    Qed.
 
   End env.
-End SepExprType.
 
-Module Make (ST' : SepTheoryX.SepTheoryXType) <: SepExprType with Module ST := ST'.
+  (** TODO: Fix this so that it works consistently! **)
+  Ltac heq_canceler :=
+    let cancel cp ap1 ap2 ep cc ac1 ac2 ec frm P Q :=
+      let rec iter_right Q :=
+        match Q with 
+          | SE.Emp =>
+            apply ec
+          | SE.Star ?L ?R =>
+            (apply ac1 ; iter_right L) || (apply ac2 ; iter_right R)
+          | _ => 
+            apply frm; [ reflexivity | ]
+        end
+      in
+      let rec iter_left P :=
+        match P with
+          | SE.Emp =>
+            apply ep
+          | SE.Star ?L ?R =>
+            (apply ap1 ; iter_left L) || (apply ap2 ; iter_left R)
+          | _ => 
+            match Q with
+              | SE.Star ?A ?B =>
+                iter_right A || (apply cc; iter_right B)
+            end
+        end
+      in
+      match P with 
+        | SE.Star ?A ?B =>
+          iter_left A || (apply cp; iter_left B)
+      end
+    in
+    repeat (rewrite heq_star_emp_l || rewrite heq_star_emp_r) ;
+    repeat match goal with
+             | [ |- SE.heq _ _ _ _ _ ?P ?Q ] =>
+               cancel heq_star_comm_p heq_star_assoc_p1 heq_star_assoc_p2 heq_star_emp_p 
+                      heq_star_comm_c heq_star_assoc_c1 heq_star_assoc_c2 heq_star_emp_c
+                      heq_star_frame P Q
+(*    | [ |- SE.himp _ _ _ _ _ ?P ?Q ] =>
+   cancel himp_star_comm_p himp_star_assoc_p himp_star_comm_c himp_star_assoc_c P Q
+   *)
+    end; try reflexivity.
+
+(*
+  Section test.
+    Variable types : list type.
+    Variable pcType : tvar.
+    Variable stateType : tvar.
+    Variable funcs : functions types.
+    Variable preds : SE.predicates types pcType stateType.
+    
+    Variables U G : env types.
+    Variable cs : codeSpec (tvarD types pcType) (tvarD types stateType).
+
+    Goal forall P Q R T V,
+      SE.heq funcs preds U G cs 
+         (SE.Star (SE.Star Q R) (SE.Star T (SE.Star V (SE.Star P SE.Emp))))
+         (SE.Star P (SE.Star (SE.Star Q R) (SE.Star (SE.Star SE.Emp T) (SE.Star SE.Emp V)))).
+    Proof.
+      intros. heq_canceler. 
+    Qed.
+
+(*
+    Goal forall P Q R S,
+      SE.heq funcs preds U G cs 
+         (SE.Star P (SE.Star Q R))
+         (SE.Star R (SE.Star).
+    Proof.
+      intros. heq_canceler. 
+    Qed.
+*)
+  End test.
+*)      
+
+End SepExprFacts.
+
+Module Make (ST' : SepTheoryX.SepTheoryXType) <: SepExpr with Module ST := ST'.
   Module ST := ST'.
 
-  Module SEP_FACTS := SepTheoryX_Rewrites ST.
   Section env.
     Variable types : list type.
     Variable pcType : tvar.
@@ -185,935 +427,15 @@ Module Make (ST' : SepTheoryX.SepTheoryXType) <: SepExprType with Module ST := S
       (gl gr : sexpr) : Prop :=
       ST.heq cs (sexprD meta_env var_env gl) (sexprD meta_env var_env gr).
 
-    Section Facts.
-      Variables U G : env types.
-      Variable cs : codeSpec (tvarD types pcType) (tvarD types stateType).
-
-      Global Instance Trans_himp : Transitive (@himp U G cs).
-      Proof.
-        red. unfold himp. intros; etransitivity; eauto.
-      Qed.
-
-      Global Instance Trans_heq : Transitive (@heq U G cs).
-      Proof.
-        red. unfold heq. intros; etransitivity; eauto.
-      Qed.
-
-      Global Instance Refl_himp : Reflexive (@himp U G cs).
-      Proof.
-        red; unfold himp; intros. reflexivity.
-      Qed.
-
-      Global Instance Refl_heq : Reflexive (@heq U G cs).
-      Proof.
-        red; unfold heq; intros. reflexivity.
-      Qed.
-
-      Global Instance Sym_heq : Symmetric (@heq U G cs).
-      Proof.
-        red; unfold heq; intros. symmetry. auto.    
-      Qed.
-
-      Global Instance Equiv_heq : Equivalence (heq U G cs).
-      Proof.
-        constructor; eauto with typeclass_instances.
-      Qed.
-
-      Add Parametric Relation : sexpr (@himp U G cs)
-        reflexivity proved by  Refl_himp
-        transitivity proved by Trans_himp
-      as himp_rel.
-
-      Add Parametric Relation : sexpr (@heq U G cs)
-        reflexivity proved by  Refl_heq
-        symmetry proved by Sym_heq
-        transitivity proved by Trans_heq
-      as heq_rel.
-
-      Global Add Parametric Morphism : Star with
-        signature (himp U G cs ==> himp U G cs ==> himp U G cs)      
-        as star_himp_mor.
-        unfold himp; simpl; intros; eapply SEP_FACTS.star_himp_mor; eauto.
-      Qed.
-
-      Global Add Parametric Morphism : Star with
-        signature (heq U G cs ==> heq U G cs ==> heq U G cs)      
-        as star_heq_mor.
-        unfold himp; simpl; intros; eapply SEP_FACTS.star_heq_mor; eauto.
-      Qed.
-
-      Global Add Parametric Morphism : (himp U G cs) with 
-        signature (heq U G cs ==> heq U G cs ==> Basics.impl)
-        as himp_heq_mor.
-        unfold heq; simpl; intros. eapply SEP_FACTS.himp_heq_mor; eauto.
-      Qed.
-
-      Global Add Parametric Morphism : (himp U G cs) with 
-        signature (himp U G cs --> himp U G cs ++> Basics.impl)
-        as himp_himp_mor.
-        unfold himp; simpl; intros. eapply SEP_FACTS.himp_himp_mor; eauto.
-      Qed.
-
-      Global Add Parametric Morphism : (sexprD U G) with 
-        signature (heq U G cs ==> ST.heq cs)
-        as heq_ST_heq_mor.
-        unfold heq; simpl; auto.
-      Qed.
-
-      Lemma heq_star_emp_r : forall P, 
-        heq U G cs (Star P Emp) P.
-      Proof.
-        unfold heq; simpl; intros; autorewrite with hprop; reflexivity.
-      Qed.
-
-      Lemma heq_star_emp_l : forall P, 
-        heq U G cs (Star Emp P) P.
-      Proof.
-        unfold heq; simpl; intros; autorewrite with hprop; reflexivity.
-      Qed.
-
-      Lemma heq_star_assoc : forall P Q R, 
-        heq U G cs (Star (Star P Q) R) (Star P (Star Q R)).
-      Proof.
-        unfold heq; simpl; intros; autorewrite with hprop. rewrite ST.heq_star_assoc. reflexivity.
-      Qed.
-
-      Lemma heq_star_comm : forall P Q, 
-        heq U G cs (Star P Q) (Star Q P).
-      Proof.
-        unfold heq; simpl; intros; apply ST.heq_star_comm.
-      Qed.
-
-      Lemma heq_star_frame : forall P Q R S, 
-        heq U G cs P R ->
-        heq U G cs Q S ->
-        heq U G cs (Star P Q) (Star R S).
-      Proof.
-        unfold heq; simpl; intros. eapply ST.heq_star_frame; auto.
-      Qed.
-      
-      Lemma himp_star_frame : forall a c cs P Q R S,
-        himp a c cs P R ->
-        himp a c cs Q S ->
-        himp a c cs (Star P Q) (Star R S).
-      Proof.
-        unfold himp; simpl; intros. rewrite H; rewrite H0; reflexivity.
-      Qed.
-        
-    End Facts.
-
-    Lemma fold_left_star : forall T a c cs F (ls : list T)  base,
-      heq a c cs (fold_left (fun acc x => Star (F x) acc) ls base)
-      (Star (fold_left (fun acc x => Star (F x) acc) ls Emp) base).
-    Proof.
-      induction ls; simpl; intros.
-      rewrite heq_star_emp_l. reflexivity.
-      rewrite IHls. symmetry. rewrite IHls.
-      repeat rewrite heq_star_assoc. rewrite heq_star_emp_l. reflexivity.
-    Qed.
-
-    Ltac heq_fold_left_opener :=
-      match goal with
-        | [ |- context [ fold_left _ _ ?B ] ] =>
-          match B with
-            | Emp => fail 1 
-            | _ => rewrite fold_left_star with (base := B)
-          end
-      end.
-    Ltac heq_canceler :=
-      repeat (repeat rewrite heq_star_assoc; first [ apply heq_star_frame; [ reflexivity | try reflexivity ] | 
-        rewrite heq_star_comm; symmetry ]).
-
-    Existing Instance himp_rel_relation.
-    Existing Instance heq_rel_relation.
-    Hint Rewrite heq_star_emp_l heq_star_emp_r : hprop.
-
-    Theorem ST_himp_himp : forall (U G : env types) cs L R,
-      himp U G cs L R ->
-      ST.himp cs (sexprD U G L) (sexprD U G R).
-    Proof.
-      clear. auto.
-    Qed.
-
-    Theorem ST_heq_heq : forall (U G : env types) cs L R,
-      heq U G cs L R ->
-      ST.heq cs (sexprD U G L) (sexprD U G R).
-    Proof.
-      clear. auto.
-    Qed.
-
-    (** A more efficient representation for sexprs. **)
-    Record SHeap : Type :=
-    { impures : MM.mmap (exprs types)
-    ; pures   : list (expr types)
-    ; other   : list (ST.hprop (tvarD types pcType) (tvarD types stateType) nil)
-    }.
-  
-    Definition SHeap_empty : SHeap := 
-      {| impures := @MM.empty _
-       ; pures   := nil
-       ; other   := nil
-       |}.
-
-    (** lift all the "real" variables in [a,...) 
-     ** to the range [a+b,...)
-     **)
-    Fixpoint liftSExpr (a b : nat) (s : sexpr) : sexpr :=
-      match s with
-        | Emp => Emp
-        | Inj p => Inj (liftExpr a b p)
-        | Star l r => Star (liftSExpr a b l) (liftSExpr a b r)
-        | Exists t s => 
-          Exists t (liftSExpr (S a) b s)
-        | Func f xs => Func f (map (liftExpr a b) xs)
-        | Const c => Const c
-      end.
-
-    (** lift all the "real" variables in [a,...) 
-     ** to the range [a+b,...)
-     **)
-    Definition liftSHeap (a b : nat) (s : SHeap) : SHeap :=
-      {| impures := MM.mmap_map (map (liftExpr a b)) (impures s)
-       ; pures   := map (liftExpr a b) (pures s)
-       ; other   := other s
-       |}.
-
-    Fixpoint star_SHeap (l r : SHeap) : SHeap :=
-      {| impures := MM.mmap_join (impures l) (impures r)
-       ; pures := pures l ++ pures r
-       ; other := other l ++ other r
-       |}.
-
-    Definition sheap_liftVars (from : nat) (delta : nat) (h : SHeap) : SHeap :=
-      {| impures := MM.mmap_map (map (liftExpr from delta)) (impures h)
-       ; pures := map (liftExpr from delta) (pures h)
-       ; other := other h
-       |}.
-
-    (** CURRENTLY NOT USED **)
-    Fixpoint substV types (vs : list nat) (e : expr types) : expr types :=
-      match e with
-        | Expr.Const _ c => Expr.Const c
-        | Var x => 
-          Var (match nth_error vs x with
-                 | None => x
-                 | Some y => y
-               end)
-        | UVar x => UVar x
-        | Expr.Func f xs => 
-          Expr.Func f (map (substV vs) xs)
-        | Equal t e1 e2 => Equal t (substV vs e1) (substV vs e2)
-        | Not e1 => Not (substV vs e1)
-      end.
-
-    Fixpoint hash (s : sexpr) : ( variables * SHeap ) :=
-      match s with
-        | Emp => (nil, SHeap_empty)
-        | Inj p => (nil,
-          {| impures := MM.empty _
-           ; pures := p :: nil
-           ; other := nil
-           |})
-        | Star l r =>
-          let (vl, hl) := hash l in
-          let (vr, hr) := hash r in
-          let nr := length vr in
-          (vl ++ vr,
-            star_SHeap (sheap_liftVars 0 nr hl) (sheap_liftVars nr (length vl) hr))
-        | Exists t b =>
-          let (v, b) := hash b in
-          (t :: v, b)
-        | Func f a =>
-          (nil,
-           {| impures := MM.mmap_add f a (MM.empty _)
-            ; pures := nil
-            ; other := nil
-           |})
-        | Const c => 
-          (@nil tvar,
-           {| impures := MM.empty _
-            ; pures := @nil (expr types)
-            ; other := c :: nil
-            |})
-      end.
-
-    Definition starred (T : Type) (F : T -> sexpr) (ls : list T) (base : sexpr)
-      : sexpr :=
-      fold_right (fun x a => match a with 
-                               | Emp => F x
-                               | _ => Star (F x) a
-                             end) base ls.
-
-    Definition sheapD (h : SHeap) : sexpr :=
-      let a := starred (fun x => Const x) (other h) Emp in
-      let a := starred (fun x => Inj x) (pures h) a in
-      let a := MM.FM.fold (fun k => starred (Func k)) (impures h) a in
-      a.
-
-    Definition starred' (T : Type) (F : T -> sexpr) (ls : list T) (base : sexpr)
-      : sexpr :=
-      fold_right (fun x a => Star (F x) a) base ls.
-
-    Definition impuresD' (imp : MM.mmap (exprs types)) : sexpr :=
-      MM.FM.fold (fun k ls acc => 
-        Star (starred' (Func k) ls Emp) acc) imp Emp.
-
-    Definition sheapD' (h : SHeap) :  sexpr :=
-      let a := MM.FM.fold (fun k ls acc => 
-        Star (starred' (Func k) ls Emp) acc) (impures h) Emp in
-      let c := starred' (fun x => Inj x) (pures h) Emp in
-      let e := starred' (fun x => Const x) (other h) Emp in
-      Star a (Star c e).
-
-    Lemma starred_starred' : forall a c cs T F F' base base' ls, 
-      heq a c cs base base' ->
-      (forall x, heq a c cs (F x) (F' x)) ->
-      heq a c cs (@starred T F ls base) (@starred' T F' ls base').
-    Proof.
-      induction ls; simpl; intros.
-        assumption.
-        specialize (IHls H H0).
-        etransitivity. instantiate (1 := (Star (F a0) (starred F ls base))).
-        destruct (starred F ls base); try reflexivity.
-        autorewrite with hprop. reflexivity.
-        rewrite H0. rewrite IHls. reflexivity.
-    Qed.
-
-    Lemma starred'_base : forall a c cs T F base ls, 
-      heq a c cs (Star (@starred' T F ls Emp) base) (@starred' T F ls base).
-    Proof.
-      unfold heq in *; simpl in *.
-      induction ls; simpl; intros.
-        autorewrite with hprop; reflexivity.
-        rewrite <- IHls. rewrite ST.heq_star_assoc. reflexivity.
-    Qed.
-
-    Lemma starred_base : forall a c cs T F base ls, 
-      heq a c cs (Star (@starred T F ls Emp) base) (@starred T F ls base).
-    Proof.
-      unfold heq in *; simpl in *.
-      induction ls; simpl; intros.
-        autorewrite with hprop; reflexivity.
-        Opaque exprD.
-        destruct (starred F ls base); destruct (starred F ls Emp);
-          simpl in *; autorewrite with hprop in *; try rewrite ST.heq_star_assoc; try rewrite IHls;
-            autorewrite with hprop; try reflexivity.
-    Qed.
-
-    Global Add Parametric Morphism a c cs : (fun k0 : nat => starred (Func k0)) with
-      signature (eq ==> eq ==> heq a c cs ==> heq a c cs)
-      as star_himp_mor'.
-    Proof.
-      intros.
-      repeat match goal with
-               | [ |- Morphisms.Proper _ _ ] => red; intros; subst
-               | [ |- Morphisms.respectful _ _ _ _ ] => red; intros; subst
-               | [ H : heq _ _ _ _ _ |- _ ] => rewrite H; clear H
-               | [ |- heq _ _ _ _ ] => heq_canceler
-             end.
-      rewrite <- starred_base. symmetry. rewrite <- starred_base. heq_canceler.
-      symmetry; auto.
-    Qed.
-    Lemma transpose_neqkey_starred a c cs : NatMap.IntMapProperties.transpose_neqkey (heq a c cs)
-      (fun k0 : nat => starred (Func k0)).
-    Proof.
-      red. intros. rewrite <- starred_base. symmetry.
-      rewrite <- starred_base. repeat rewrite <- starred_base with (base := a0).
-      heq_canceler.
-    Qed.
-    Lemma transpose_neqkey_Star (X : Type) F a c cs : NatMap.IntMapProperties.transpose_neqkey (heq a c cs)
-      (fun (k0 : nat) (ls : X) (a1 : sexpr) => Star (F k0 ls) a1).
-    Proof.
-      red. intros. heq_canceler.
-    Qed.
-    Hint Resolve transpose_neqkey_starred transpose_neqkey_Star : hprop.
-    Hint Extern 1 (Morphisms.Proper _ _) =>
-      (unfold Morphisms.Proper, Morphisms.respectful; intros; subst; 
-        repeat match goal with
-                 | [ H : heq _ _ _ _ _ |- _ ] => rewrite H
-               end; reflexivity) : hprop.
-    Hint Extern 1 (MM.PROPS.transpose_neqkey _ _) => 
-      (clear; repeat (red; intros; subst); repeat rewrite MM.FACTS.add_o;
-        repeat match goal with 
-                 | [ |- context [ FM.E.eq_dec ?X ?Y ] ] => 
-                   destruct (FM.E.eq_dec X Y)
-                 | [ H : FM.E.eq ?X ?Y |- _ ] => rewrite H in *
-               end; solve [ auto | exfalso; auto | heq_canceler ]) : hprop.
-
-    Lemma fold_starred : forall X a c cs (F : nat -> X -> sexpr) m b,
-      heq a c cs (MM.FM.fold (fun k ls a => Star (F k ls) a) m b)
-      (Star (MM.FM.fold (fun k ls a => Star (F k ls) a) m Emp) b).
-    Proof.
-      do 5 intro.
-      intro. apply NatMap.IntMapProperties.fold_rec with (m := m).
-        intros. rewrite NatMap.IntMapProperties.fold_Empty; eauto with typeclass_instances.
-        autorewrite with hprop. reflexivity.
-
-        intros. erewrite NatMap.IntMapProperties.fold_Add; eauto with typeclass_instances hprop.
-        rewrite H2. heq_canceler.
-    Qed.
-
-    Lemma impures' : forall a c cs (i : MM.mmap _)  b, 
-      heq a c cs (MM.FM.fold (fun k => starred (Func k)) i b)
-      (Star (MM.FM.fold (fun k ls a => Star (starred' (Func k) ls Emp) a) i Emp) b).
-    Proof.
-      do 4 intro. apply NatMap.IntMapProperties.fold_rec with (m := i); intros.
-        rewrite NatMap.IntMapProperties.fold_Empty; eauto with typeclass_instances.
-        autorewrite with hprop; reflexivity.
-
-        erewrite NatMap.IntMapProperties.fold_Add; eauto with typeclass_instances hprop.
-        rewrite <- starred_base. rewrite starred_starred'; try reflexivity.
-        rewrite H2. heq_canceler.
-    Qed.
-
-    Theorem sheapD_sheapD' : forall a c cs h, 
-      heq a c cs (sheapD h) (sheapD' h).
-    Proof.
-      destruct h; unfold sheapD, sheapD'; simpl.
-      rewrite impures'. rewrite <- (@starred_base a c cs). 
-      rewrite <- (@starred_base a c cs) with (ls := other0).
-      eapply heq_star_frame. reflexivity.
-      eapply heq_star_frame. eapply starred_starred'; reflexivity.
-      autorewrite with hprop.
-      eapply starred_starred'; reflexivity.
-    Qed.
-
-    Lemma starred_In : forall T (F : T -> sexpr) a c cs x ls' b ls,
-      heq a c cs (starred F (ls ++ x :: ls') b) (Star (starred F (ls ++ ls') b) (F x)).
-    Proof.
-      induction ls; intros.
-        symmetry; rewrite heq_star_comm.
-        repeat rewrite starred_starred' by reflexivity.
-        reflexivity.
-
-        generalize dependent IHls.
-        repeat rewrite starred_starred' by reflexivity.
-        intro IHls. simpl. rewrite heq_star_assoc.
-        rewrite IHls. reflexivity.
-    Qed.
-
-    Lemma sheapD_pures : forall stn sm cs uvars vars h,
-      ST.satisfies cs (sexprD uvars vars (sheapD h)) stn sm ->
-      AllProvable funcs uvars vars (pures h).
-    Proof.
-      intros. eapply ST.satisfies_himp in H.
-      Focus 2. instantiate (1 := sexprD uvars vars (sheapD' h)). 
-      match goal with
-        | [ |- ?G ] => 
-          change G with (himp uvars vars cs (sheapD h) (sheapD' h))
-      end.
-      rewrite sheapD_sheapD'. reflexivity.
-      
-      destruct h. unfold sheapD' in *.
-      eapply ST.satisfies_himp in H.
-      Focus 2.
-      instantiate (1 := sexprD uvars vars
-           (Star
-              (starred' (fun x : expr types => Inj x)
-                 (pures
-                    {|
-                    impures := impures0;
-                    pures := pures0;
-                    other := other0 |}) Emp)
-
-        (Star
-           (MM.FM.fold
-              (fun (k : nat) (ls : list (list (expr types)))
-                 (acc : sexpr) =>
-               Star (starred' (Func k) ls Emp) acc)
-              (impures
-                 {| impures := impures0; pures := pures0; other := other0 |})
-              Emp)
-              (starred'
-                 (fun
-                    x : ST.hprop (tvarD types pcType) 
-                          (tvarD types stateType) nil => 
-                  Const x)
-                 (other
-                    {|
-                    impures := impures0;
-                    pures := pures0;
-                    other := other0 |}) Emp)))).
-      match goal with
-        | [ |- ST.himp ?C (sexprD ?U ?V ?L) (sexprD ?U ?V ?R) ] =>
-          change (ST.himp C (sexprD U V L) (sexprD U V R)) with
-            (himp U V C L R)
-      end.
-
-      simpl. rewrite heq_star_comm. rewrite heq_star_assoc.
-      apply himp_star_frame; try reflexivity. rewrite heq_star_comm.
-      reflexivity.
-      
-      match goal with
-        | [ H : ST.satisfies _ (sexprD _ _ (Star _ ?X)) _ _ |- _ ] =>
-          generalize dependent X
-      end.
-      simpl. clear.
-      
-      generalize sm. clear.
-      induction pures0; simpl; intros; auto.
-        rewrite ST.heq_star_assoc in H.
-        apply ST.satisfies_star in H. do 2 destruct H.
-        intuition eauto.
-        unfold Provable. destruct (exprD funcs uvars vars a tvProp);
-        apply ST.satisfies_pure in H; propxFo.
-    Qed.
-
-    Lemma sheapD_pull_impure : forall a c cs h f argss,
-      MM.FM.find f (impures h) = Some argss ->
-      heq a c cs (sheapD h)
-                 (Star (sheapD {| impures := MM.FM.remove f (impures h)
-                                ; pures   := pures h
-                                ; other   := other h |})
-                       (starred (Func f) argss Emp)).
-    Proof.
-      intros. 
-      repeat rewrite sheapD_sheapD'.
-      unfold sheapD'; destruct h; simpl.
-      etransitivity.
-      eapply heq_star_frame. 2: reflexivity.      
-      instantiate (1 := (Star
-         (MM.FM.fold
-            (fun (k : nat) (ls : list (list (expr types)))
-               (acc : sexpr) =>
-             Star (starred' (Func k) ls Emp) acc) (MM.FM.remove f impures0) Emp)
-         (starred (Func f) argss Emp))).
-      Focus 2.
-      rewrite heq_star_assoc. rewrite heq_star_comm. rewrite heq_star_assoc.
-      rewrite heq_star_comm. rewrite heq_star_assoc.
-      symmetry. rewrite heq_star_assoc. rewrite heq_star_comm.
-      heq_canceler.
-
-      rewrite NatMap.IntMapProperties.fold_Add with (m2 := impures0); eauto with typeclass_instances hprop.
-      Focus 3. unfold NatMap.IntMapProperties.Add. instantiate (3 := f). instantiate (2 := argss).
-      instantiate (1 := (MM.FM.remove f impures0)). intros.
-        rewrite NatMap.IntMapProperties.F.add_o. simpl in *.
-        destruct (NatMap.Ordered_nat.eq_dec f y). subst; auto.
-        rewrite NatMap.IntMapProperties.F.remove_neq_o; auto.
-
-      Focus 2. apply MM.FM.remove_1; auto.
-
-      rewrite starred_starred'; try reflexivity. heq_canceler.
-    Qed.
-
-    Lemma heq_ex : forall X Y cs t P Q,
-      (forall v : tvarD types t, heq X (existT (tvarD types) t v :: Y) cs P Q) ->
-      heq X Y cs (Exists t P) (Exists t Q).
-    Proof.
-      unfold heq; simpl; intros; apply ST.heq_ex; auto.
-    Qed.
-
-    (** The first variable in the list is the first one quantified!
-     **)
     Fixpoint existsEach (ls : list tvar) {struct ls} : sexpr -> sexpr :=
       match ls with
         | nil => fun x => x
         | t :: ts => fun y => Exists t (@existsEach ts y)
       end.
-    
-    Lemma heq_existsEach : forall cs X v Y (P Q : sexpr),
-      (forall Z, map (@projT1 _ _) Z = rev v -> heq X (Z ++ Y) cs P Q) ->
-      heq X Y cs (existsEach v P) (existsEach v Q).
-    Proof.
-      induction v; simpl; intros.
-        specialize (H nil); simpl in *; auto.
-
-        apply heq_ex. intros. eapply IHv. intros.
-        simpl. specialize (H (Z ++ @existT _ _ _ v0 :: nil)). rewrite map_app in *. 
-        rewrite H0 in *. simpl in *.
-        rewrite app_ass in *. simpl in *. auto.
-    Qed.
-
-    Lemma existsEach_app : forall X cs b a Y (P : sexpr),
-      heq X Y cs (existsEach a (existsEach b P)) (existsEach (a ++ b) P).
-    Proof.
-      induction a; simpl.
-        reflexivity.
-        intros. apply heq_ex; intros. apply IHa.
-    Qed.
-
-    Lemma liftSExpr_0 : forall b a, liftSExpr a 0 b = b.
-    Proof.
-      induction b; simpl; intros; auto.
-      rewrite liftExpr_0; reflexivity.
-      rewrite IHb1; rewrite IHb2; reflexivity.
-      rewrite IHb. auto.
-      f_equal. clear. induction l; simpl; auto. rewrite liftExpr_0. f_equal; auto.
-    Qed.
-    
-    Lemma sexpr_lift_ext : forall EG cs G G' s G'',
-      ST.heq cs (sexprD EG (G'' ++ G) s) (sexprD EG (G'' ++ G' ++ G) (liftSExpr (length G'') (length G') s)).
-    Proof.
-      induction s; simpl; intros; 
-        repeat match goal with
-                 | [ |- _ ] => rewrite <- liftExpr_ext
-                 | [ H : forall a, ST.heq _ _ _ |- _ ] => rewrite <- H
-               end; try reflexivity.
-      eapply ST.heq_ex. intros. specialize (IHs (existT (tvarD types) t v :: G'')).
-      simpl in *. auto.
-      destruct (nth_error sfuncs f); try reflexivity.
-      clear. destruct s; simpl; clear. generalize dependent SDomain0. induction l; simpl; try reflexivity.
-      destruct SDomain0; try reflexivity.
-      rewrite <- liftExpr_ext. destruct (exprD funcs EG (G'' ++ G) a t); try reflexivity.
-      auto.
-    Qed.
-
-    Lemma star_pull_exists : forall EG cs a G s s2,
-      heq EG G cs (Star (Exists a s) s2) (Exists a (Star s (liftSExpr 0 1 s2))).
-    Proof.
-      intros. unfold heq. simpl. rewrite ST.heq_ex_star. apply ST.heq_ex. intros.
-      apply ST.heq_star_cancel.
-      generalize (sexpr_lift_ext EG cs G (existT (tvarD types) a v :: nil) s2 nil); simpl; intro. auto.
-    Qed.            
-
-    Lemma liftSExpr_combine : forall s a b c,
-      liftSExpr a b (liftSExpr a c s) = liftSExpr a (c + b) s.
-    Proof.
-      clear. induction s; intros; simpl; 
-      repeat match goal with
-               | [ H : _ |- _ ] => rewrite H
-             end; try reflexivity. 
-      rewrite liftExpr_combine. reflexivity.
-      f_equal. rewrite map_map. apply map_ext. intros; apply liftExpr_combine.
-    Qed.
-
-    Lemma star_pull_existsEach : forall EG cs v G s s2,
-      heq EG G cs (Star (existsEach v s) s2)
-      (existsEach v (Star s (liftSExpr 0 (length v) s2))).
-    Proof.
-      induction v; simpl.
-      intros; rewrite liftSExpr_0. reflexivity.
-
-      intros.
-      rewrite star_pull_exists. apply heq_ex. intros.
-      rewrite IHv.
-     
-      rewrite liftSExpr_combine. reflexivity.
-    Qed.
-
-    Lemma starred'_app : forall EG G cs T (F : T -> _) a b B,
-      heq EG G cs (starred' F (a ++ b) B) (starred' F a (starred' F b B)).
-    Proof.
-      induction a; simpl; intros; try reflexivity.     
-      rewrite IHa. reflexivity.
-    Qed.
-
-    Lemma add_remove_Equal : forall (elt : Type) k (v : elt) m,
-      MM.FM.Equal (MM.FM.add k v m) (MM.FM.add k v (MM.FM.remove k m)).
-    Proof.
-      clear. unfold MM.FM.Equal. intros.
-      repeat (rewrite NatMap.IntMapFacts.add_o || rewrite NatMap.IntMapFacts.remove_o).
-      destruct (NatMap.Ordered_nat.eq_dec k y); auto.
-    Qed.
-
-    Lemma multimap_join_star : forall (EG G : env types)
-     (cs : codeSpec (tvarD types pcType) (tvarD types stateType))
-     (impures0 impures1 : MM.mmap (exprs types)) B,
-     heq EG G cs
-       (MM.FM.fold
-         (fun (k : nat) (ls : list (exprs types)) (acc : sexpr) =>
-           Star (starred' (Func k) ls Emp) acc)
-         (MM.mmap_join impures0 impures1) B)
-       (MM.FM.fold
-         (fun (k : nat) (ls : list (exprs types)) (acc : sexpr) =>
-           Star (starred' (Func k) ls Emp) acc) impures0 
-         (MM.FM.fold
-           (fun (k : nat) (ls : list (exprs types)) (acc : sexpr) =>
-             Star (starred' (Func k) ls Emp) acc) impures1 B)).
-    Proof.
-      unfold MM.mmap_join.
-      do 4 intro. apply NatMap.IntMapProperties.map_induction with (m := impures0).
-      * intros.
-        repeat rewrite NatMap.IntMapProperties.fold_Empty with (m := m); eauto with typeclass_instances.
-        reflexivity.
-
-      * intros.
-        generalize (@NatMap.IntMapProperties.fold_Add (list (exprs types)) _ (@MM.FM.Equal (list (exprs types)))).
-        intro. 
-        rewrite NatMap.IntMapProperties.fold_Equal; try solve [ clear; eauto with typeclass_instances ].
-        4: eapply H2; eauto with typeclass_instances.
-        clear H2. simpl in *.
-        unfold exprs, MM.mmap_extend; simpl in *.
-        match goal with
-          | [ |- context [ MM.FM.find ?x ?y ] ] => remember y
-        end.
-        case_eq (MM.FM.find x t); intros.
-        { subst.
-          rewrite NatMap.IntMapProperties.fold_Equal; eauto with typeclass_instances.
-          4: eapply add_remove_Equal.
-          symmetry.
-          rewrite NatMap.IntMapProperties.fold_Add.
-          6: eassumption.
-          5: eauto.
-          2: eauto with typeclass_instances.
-          rewrite fold_starred.
-          rewrite NatMap.IntMapProperties.fold_Add with (m2 := impures1).
-          2: eauto with typeclass_instances.
-          instantiate (3 := x). instantiate (2 := l). 
-          instantiate (1 := MM.FM.remove x impures1). 
-          rewrite NatMap.IntMapProperties.fold_add.
-          rewrite starred'_app. rewrite <- starred'_base with (base := starred' _ _ _).
-          repeat rewrite heq_star_assoc. apply heq_star_frame; try reflexivity.
-          rewrite heq_star_comm. repeat rewrite heq_star_assoc. apply heq_star_frame; try reflexivity.
-          
-          generalize (@MM.mmap_join_remove_acc _ x m impures1 H0). unfold MM.mmap_join. intro.
-          symmetry. rewrite NatMap.IntMapProperties.fold_Equal.
-          5: eapply H3. clear H3.
-          rewrite H. rewrite fold_starred with (b := MM.FM.fold _ _ _). heq_canceler. eauto with typeclass_instances.
-            
-            try solve [ clear; eauto with typeclass_instances | clear; repeat (red; intros; subst); try rewrite H; heq_canceler ].
-            try solve [ clear; eauto with typeclass_instances | clear; repeat (red; intros; subst); try rewrite H; heq_canceler ].
-            try solve [ clear; eauto with typeclass_instances | clear; repeat (red; intros; subst); try rewrite H; heq_canceler ].
-            try solve [ clear; eauto with typeclass_instances | clear; repeat (red; intros; subst); try rewrite H; heq_canceler ].
-            try solve [ clear; eauto with typeclass_instances | clear; repeat (red; intros; subst); try rewrite H; heq_canceler ].
-            apply MM.FM.remove_1; auto.
-            try solve [ clear; eauto with typeclass_instances | clear; repeat (red; intros; subst); try rewrite H; heq_canceler ].
-            try solve [ clear; eauto with typeclass_instances | clear; repeat (red; intros; subst); try rewrite H; heq_canceler ].
-            apply MM.FM.remove_1; auto.
-
-            { 
-              generalize MM.mmap_join_o. 
-              unfold MM.mmap_join. intros. unfold MM.mmap_extend in H3. rewrite H3 in H2; auto. 
-              apply MM.PROPS.F.not_find_in_iff in H0. unfold exprs in H0. rewrite H0 in H2.
-              
-              revert H2; clear; intros.
-              unfold NatMap.IntMapProperties.Add; intros.
-                repeat (rewrite NatMap.IntMapFacts.add_o || rewrite NatMap.IntMapFacts.remove_o).
-                destruct (NatMap.Ordered_nat.eq_dec x y); subst; auto.
-            }
-
-            try solve [ clear; eauto with typeclass_instances | clear; repeat (red; intros; subst); try rewrite H; heq_canceler ].
-            try solve [ clear; eauto with typeclass_instances | clear; repeat (red; intros; subst); try rewrite H; heq_canceler ].
-            try solve [ clear; eauto with typeclass_instances | clear; repeat (red; intros; subst); try rewrite H; heq_canceler ].
-            try solve [ clear; eauto with typeclass_instances | clear; repeat (red; intros; subst); try rewrite H; heq_canceler ].
-        }          
-        { subst.
-          rewrite NatMap.IntMapProperties.fold_add; eauto with typeclass_instances.
-          rewrite H. symmetry. rewrite fold_starred. 
-          rewrite NatMap.IntMapProperties.fold_Add; eauto with typeclass_instances.
-          symmetry. rewrite fold_starred with (b := MM.FM.fold _ _ _). heq_canceler.
-          
-          repeat (red; intros; subst). rewrite H3. heq_canceler.
-          red; intros; heq_canceler.
-          repeat (red; intros; subst). rewrite H3; heq_canceler.
-          red; intros; heq_canceler.
-          intro.
-          apply NatMap.IntMapProperties.F.in_find_iff in H3. auto.
-        }
-        eauto with typeclass_instances.
-        try solve [ clear; eauto with typeclass_instances | clear; repeat (red; intros; subst); try rewrite H; heq_canceler ].
-        try solve [ clear; eauto with typeclass_instances | clear; repeat (red; intros; subst); try rewrite H; heq_canceler ].
-        clear; repeat (red; intros; subst). unfold MM.mmap_extend. rewrite H.
-          destruct (MM.FM.find (elt:=list (exprs types)) y y1); try rewrite H; reflexivity.
-
-        eapply MM.transpose_neqkey_mmap_extend.
-    Qed.
-
-
-    Lemma sheapD'_star : forall EG G cs s1 s2,
-      heq EG G cs (sheapD' (star_SHeap s1 s2)) (Star (sheapD' s1) (sheapD' s2)).
-    Proof.
-      destruct s1; destruct s2; intros; simpl; unfold sheapD', star_SHeap; simpl.
-      match goal with
-        | [ |- heq _ _ _ _ (Star (Star ?FL (Star ?PL ?OL)) (Star ?FR (Star ?PR ?OR))) ] =>
-          transitivity (Star (Star FL FR) (Star (Star PL PR) (Star OL OR)))
-      end.
-      repeat apply heq_star_frame.
-      Focus.
-      rewrite multimap_join_star; auto. 
-      repeat rewrite MM.FM.fold_1; auto.
-      rewrite fold_left_star. reflexivity.
-
-      (** **)
-      clear; induction pures0; simpl.
-        rewrite heq_star_emp_l. reflexivity.
-        rewrite heq_star_assoc. rewrite IHpures0. reflexivity.
-
-      clear; induction other0; simpl.
-        rewrite heq_star_emp_l; reflexivity.
-        rewrite heq_star_assoc. rewrite IHother0. reflexivity.
-
-      repeat (repeat rewrite heq_star_assoc; repeat (eapply heq_star_frame; [ reflexivity | ]); rewrite heq_star_comm).
-      (repeat rewrite heq_star_assoc; repeat (eapply heq_star_frame; [ reflexivity | ])). reflexivity.
-    Qed.
-
-    Lemma fold_left_Star : forall T EG G cs (F : T -> _) ls base base',
-      heq EG G cs base base' ->
-      heq EG G cs (fold_left (fun acc x => Star (F x) acc) ls base)
-      (fold_left (fun acc x => Star (F x) acc) ls base').
-    Proof.
-      induction ls; simpl; intros; auto.
-      rewrite IHls. reflexivity. apply heq_star_frame; auto; reflexivity.
-    Qed.
-
-    Lemma starred'_liftSExpr : forall EG G cs F a b (ls : list (expr types)) base,
-      (forall a0, heq EG G cs (liftSExpr a b (F a0)) (F (liftExpr a b a0))) ->
-      heq EG G cs
-      (liftSExpr a b (starred' F ls base))
-      (starred' F (map (liftExpr a b) ls) (liftSExpr a b base)).
-    Proof.
-      induction ls; simpl; intros; try reflexivity.
-      rewrite IHls. rewrite H. reflexivity. eauto.
-    Qed.
-
-    Lemma liftSExpr_existsEach : forall EG cs v0 s G n v,
-      heq EG G cs (liftSExpr n v (existsEach v0 s)) 
-                  (existsEach v0 (liftSExpr (n + length v0) v s)).
-    Proof.
-      induction v0; simpl; intros.
-        intros. rewrite Plus.plus_0_r. reflexivity.
-      
-        apply heq_ex; intros. rewrite IHv0. cutrewrite (S n + length v0 = n + S (length v0)); try reflexivity; omega.
-    Qed.
-
-    Lemma skipn_skipn : forall T a (ls : list T) b,
-      skipn b (skipn a ls) = skipn (b + a) ls.
-    Proof.
-      clear; induction a; simpl; intros.
-        rewrite Plus.plus_0_r. auto.
-        rewrite Plus.plus_comm. simpl. destruct ls; auto. destruct b; auto.
-        rewrite IHa. rewrite Plus.plus_comm. auto.
-    Qed.
-
-    Lemma heq_liftSExpr : forall cs EG G G' G'' P Q,
-      heq EG (G ++ G'') cs P Q ->
-      heq EG (G ++ G' ++ G'') cs (liftSExpr (length G) (length G') P) (liftSExpr (length G) (length G') Q).
-    Proof.
-      unfold heq; intros.
-      repeat rewrite <- sexpr_lift_ext. auto.
-    Qed.
-
-    Lemma sheapD'_sexprD_liftVars : forall EG cs s G G' G'',
-      heq EG (G ++ G' ++ G'') cs (liftSExpr (length G) (length G') (sheapD' s))
-                                 (sheapD' (sheap_liftVars (length G) (length G') s)).
-    Proof.
-      destruct s; unfold sheap_liftVars, sheapD'; simpl; intros; repeat apply heq_star_frame; intros;
-        try solve [ clear; induction pures0; simpl; try rewrite IHpures0; reflexivity
-                  | clear; induction other0; simpl; try rewrite IHother0; try reflexivity ].
-
-      clear. change Emp with (liftSExpr (length G) (length G') Emp) at 3 4. generalize Emp at 2 4.
-        unfold MM.mmap_map. intros. rewrite MF.fold_map_fusion; eauto with typeclass_instances hprop.
-
-        Focus. 
-        apply NatMap.IntMapProperties.map_induction with (m := impures0); intros.
-        repeat (rewrite MM.PROPS.fold_Empty; eauto with typeclass_instances). reflexivity.
-
-        symmetry. rewrite MM.PROPS.fold_Add. 6: eauto. 5: eauto. 2: eauto with typeclass_instances.
-        rewrite <- H.
-        assert (forall base, heq EG (G ++ G' ++ G'') cs 
-          (starred' (Func x) (map (map (liftExpr (length G) (length G'))) e) (liftSExpr (length G) (length G') base))
-          (liftSExpr (length G) (length G') (starred' (Func x) e base))). clear.
-          induction e; simpl; intros; try reflexivity.
-            rewrite IHe; reflexivity.
-        rewrite H2.
-        change (Star (liftSExpr (length G) (length G') (starred' (Func x) e Emp))
-        (liftSExpr (length G) (length G')
-           (MM.FM.fold
-              (fun (k : MM.FM.key) (ls : list (list (expr types)))
-                 (acc : sexpr) => Star (starred' (Func k) ls Emp) acc) m s)))
-        with (liftSExpr (length G) (length G')
-          (Star (starred' (Func x) e Emp)
-            (MM.FM.fold
-              (fun (k : MM.FM.key) (ls : list (list (expr types)))
-                (acc : sexpr) => Star (starred' (Func k) ls Emp) acc) m s))).
-
-        eapply heq_liftSExpr.
-        
-        symmetry.
-        rewrite MM.PROPS.fold_Add. 6: eauto. reflexivity.
-        eauto with typeclass_instances hprop.
-        eauto with typeclass_instances hprop.
-        eauto with typeclass_instances hprop.
-        eauto with typeclass_instances hprop.
-        eauto with typeclass_instances hprop.
-        eauto with typeclass_instances hprop.
-        clear; repeat (red; intros; subst); repeat rewrite MM.FACTS.add_o;
-          repeat match goal with 
-                   | [ |- context [ FM.E.eq_dec ?X ?Y ] ] => 
-                     destruct (FM.E.eq_dec X Y)
-                   | [ H : FM.E.eq ?X ?Y |- _ ] => rewrite H in *
-                 end; auto. heq_canceler.
-    Qed.
-
-    Lemma hash_denote' : forall EG cs (s : sexpr) G, 
-      heq EG G cs s (@existsEach (fst (hash s)) (sheapD' (snd (hash s)))).
-    Proof.
-      Opaque star_SHeap.
-      induction s; simpl; try solve [ unfold sheapD'; simpl; intros; repeat (rewrite heq_star_emp_r || rewrite heq_star_emp_l); reflexivity ].
-        (** Exists **)
-        Focus 2.
-        unfold sheapD'; simpl; intros. case_eq (hash s); intros; simpl.
-        eapply heq_ex. intros. specialize (IHs (existT (tvarD types) t v0 :: G)). simpl in *.
-        rewrite H in IHs. simpl in *. eauto.
-
-        (** Star **)
-        Focus.
-        intros. rewrite IHs1 at 1. intros.
-        destruct (hash s1); destruct (hash s2); simpl in *.
-        rewrite IHs2.
-        rewrite <- (@existsEach_app EG cs) with (Y := G).
-        rewrite star_pull_existsEach. apply heq_existsEach. intros.
-        rewrite heq_star_comm.
-
-        rewrite liftSExpr_existsEach.
-        rewrite star_pull_existsEach. eapply heq_existsEach; intros.
-        rewrite sheapD'_star. simpl plus.
-        cutrewrite (length v0 = length Z0).
-        cutrewrite (length v = length Z).
-        rewrite sheapD'_sexprD_liftVars.
-        rewrite sheapD'_sexprD_liftVars with (G := nil). heq_canceler.
-        rewrite <- rev_length; rewrite <- H; apply map_length.
-        rewrite <- rev_length; rewrite <- H0; apply map_length.
-
-        (** Func **)
-        Focus.
-        intros. unfold sheapD'. simpl. rewrite MM.FM.fold_1. simpl.
-        repeat rewrite heq_star_emp_r. reflexivity.
-    Qed.
-    
-    Theorem hash_denote : forall EG cs (s : sexpr) G, 
-      heq EG G cs s (@existsEach (fst (hash s)) (sheapD (snd (hash s)))).
-    Proof.
-      intros. specialize (@hash_denote' EG cs s G). etransitivity.
-      eassumption. apply heq_existsEach. intros. rewrite sheapD_sheapD'. reflexivity.
-    Qed.
-
-    (** replace "real" variables [a,b) and replace them with
-     ** uvars [c,..]
-     **)
-    Definition sheapSubstU (a b c : nat) (s : SHeap) : SHeap :=
-      {| impures := MM.mmap_map (map (exprSubstU a b c)) (impures s)
-       ; pures := map (exprSubstU a b c) (pures s)
-       ; other := other s
-       |}.
-
   End env.
-
-  Implicit Arguments Emp [ types pcType stateType ].
-  Implicit Arguments Star [ types pcType stateType ].
-  Implicit Arguments Exists [ types pcType stateType ].
-  Implicit Arguments Func [ types pcType stateType ].
-  Implicit Arguments Const [ types pcType stateType ].
-  Implicit Arguments Inj [ types pcType stateType ].
-
-
-  Lemma change_ST_himp_himp : forall (types : list type)
-    (funcs : functions types) (pc st : tvar)
-    (sfuncs : list (ssignature types pc st))
-    EG G
-    (cs : codeSpec (tvarD types pc) (tvarD types st))
-    (L R : sexpr types pc st),
-    himp funcs sfuncs EG G cs L R ->
-    ST.himp cs
-      (@sexprD types pc st funcs sfuncs EG G L)
-      (@sexprD types pc st funcs sfuncs EG G R).
-  Proof.
-    unfold himp. intros. auto.
-  Qed.
-
 End Make.
 
-Module ReifySepExpr (Import SEP : SepExprType).  
+Module ReifySepExpr (Import SEP : SepExpr).  
 
   (** Reflection **)
   Require Import Reflect.
@@ -1253,7 +575,7 @@ Module ReifySepExpr (Import SEP : SepExprType).
           let F := reify_sfunction pcT stT types f in
           let sfuncs := eval simpl app in (sfuncs ++ (F :: nil)) in
           k sfuncs acc
-        | ?F (*SSig _ _ _ ?F *) :: ?FS =>
+        | ?F :: ?FS =>
           match F with 
             | @SSig _ _ _ _ ?F =>
               match F with
@@ -1262,14 +584,6 @@ Module ReifySepExpr (Import SEP : SepExprType).
                   let acc := constr:(S acc) in
                   lookup FS acc
               end
-(*            | @SSig' _ _ _ ?F =>
-              match F with
-                | f => k sfuncs acc 
-                | _ => 
-                  let acc := constr:(S acc) in
-                  lookup FS acc
-              end
-*)
           end
       end
     in lookup sfuncs 0.
@@ -1290,7 +604,7 @@ Module ReifySepExpr (Import SEP : SepExprType).
    **)
   Ltac reify_sexpr isConst s types funcs pcType stateType sfuncs uvars vars k :=
     let implicits ctor :=
-      constr:(ctor types pcType stateType) (* (ST.hprop (@tvarD types pcType) (@tvarD types stateType) nil)) *)
+      constr:(ctor types pcType stateType)
     in
     let rec reflect s funcs sfuncs uvars vars k :=
       match s with
